theories/autosubst/CCAST.v
@@ -32,7 +32,11 @@ Inductive cterm : Type :=
   | etrue : cterm
   | efalse : cterm
   | bool_err : cterm
-  | eif : cmode -> cterm -> cterm -> cterm -> cterm -> cterm -> cterm.
+  | eif : cmode -> cterm -> cterm -> cterm -> cterm -> cterm -> cterm
+  | pbool : cterm
+  | ptrue : cterm
+  | pfalse : cterm
+  | pif : cterm -> cterm -> cterm -> cterm -> cterm.
 
 Lemma congr_cSort {s0 : cmode} {s1 : level} {t0 : cmode} {t1 : level}
   (H0 : s0 = t0) (H1 : s1 = t1) : cSort s0 s1 = cSort t0 t1.
@@ -217,6 +221,34 @@ exact (eq_trans
          (ap (fun x => eif t0 t1 t2 t3 t4 x) H5)).
 Qed.
 
+Lemma congr_pbool : pbool = pbool.
+Proof.
+exact (eq_refl).
+Qed.
+
+Lemma congr_ptrue : ptrue = ptrue.
+Proof.
+exact (eq_refl).
+Qed.
+
+Lemma congr_pfalse : pfalse = pfalse.
+Proof.
+exact (eq_refl).
+Qed.
+
+Lemma congr_pif {s0 : cterm} {s1 : cterm} {s2 : cterm} {s3 : cterm}
+  {t0 : cterm} {t1 : cterm} {t2 : cterm} {t3 : cterm} (H0 : s0 = t0)
+  (H1 : s1 = t1) (H2 : s2 = t2) (H3 : s3 = t3) :
+  pif s0 s1 s2 s3 = pif t0 t1 t2 t3.
+Proof.
+exact (eq_trans
+         (eq_trans
+            (eq_trans (eq_trans eq_refl (ap (fun x => pif x s1 s2 s3) H0))
+               (ap (fun x => pif t0 x s2 s3) H1))
+            (ap (fun x => pif t0 t1 x s3) H2))
+         (ap (fun x => pif t0 t1 t2 x) H3)).
+Qed.
+
 Lemma upRen_cterm_cterm (xi : nat -> nat) : nat -> nat.
 Proof.
 exact (up_ren xi).
@@ -266,6 +298,12 @@ Fixpoint ren_cterm (xi_cterm : nat -> nat) (s : cterm) {struct s} : cterm :=
       eif s0 (ren_cterm xi_cterm s1) (ren_cterm xi_cterm s2)
         (ren_cterm xi_cterm s3) (ren_cterm xi_cterm s4)
         (ren_cterm xi_cterm s5)
+  | pbool => pbool
+  | ptrue => ptrue
+  | pfalse => pfalse
+  | pif s0 s1 s2 s3 =>
+      pif (ren_cterm xi_cterm s0) (ren_cterm xi_cterm s1)
+        (ren_cterm xi_cterm s2) (ren_cterm xi_cterm s3)
   end.
 
 Lemma up_cterm_cterm (sigma : nat -> cterm) : nat -> cterm.
@@ -320,6 +358,12 @@ cterm :=
       eif s0 (subst_cterm sigma_cterm s1) (subst_cterm sigma_cterm s2)
         (subst_cterm sigma_cterm s3) (subst_cterm sigma_cterm s4)
         (subst_cterm sigma_cterm s5)
+  | pbool => pbool
+  | ptrue => ptrue
+  | pfalse => pfalse
+  | pif s0 s1 s2 s3 =>
+      pif (subst_cterm sigma_cterm s0) (subst_cterm sigma_cterm s1)
+        (subst_cterm sigma_cterm s2) (subst_cterm sigma_cterm s3)
   end.
 
 Lemma upId_cterm_cterm (sigma : nat -> cterm)
@@ -392,6 +436,14 @@ subst_cterm sigma_cterm s = s :=
         (idSubst_cterm sigma_cterm Eq_cterm s3)
         (idSubst_cterm sigma_cterm Eq_cterm s4)
         (idSubst_cterm sigma_cterm Eq_cterm s5)
+  | pbool => congr_pbool
+  | ptrue => congr_ptrue
+  | pfalse => congr_pfalse
+  | pif s0 s1 s2 s3 =>
+      congr_pif (idSubst_cterm sigma_cterm Eq_cterm s0)
+        (idSubst_cterm sigma_cterm Eq_cterm s1)
+        (idSubst_cterm sigma_cterm Eq_cterm s2)
+        (idSubst_cterm sigma_cterm Eq_cterm s3)
   end.
 
 Lemma upExtRen_cterm_cterm (xi : nat -> nat) (zeta : nat -> nat)
@@ -467,6 +519,14 @@ ren_cterm xi_cterm s = ren_cterm zeta_cterm s :=
         (extRen_cterm xi_cterm zeta_cterm Eq_cterm s3)
         (extRen_cterm xi_cterm zeta_cterm Eq_cterm s4)
         (extRen_cterm xi_cterm zeta_cterm Eq_cterm s5)
+  | pbool => congr_pbool
+  | ptrue => congr_ptrue
+  | pfalse => congr_pfalse
+  | pif s0 s1 s2 s3 =>
+      congr_pif (extRen_cterm xi_cterm zeta_cterm Eq_cterm s0)
+        (extRen_cterm xi_cterm zeta_cterm Eq_cterm s1)
+        (extRen_cterm xi_cterm zeta_cterm Eq_cterm s2)
+        (extRen_cterm xi_cterm zeta_cterm Eq_cterm s3)
   end.
 
 Lemma upExt_cterm_cterm (sigma : nat -> cterm) (tau : nat -> cterm)
@@ -540,6 +600,14 @@ subst_cterm sigma_cterm s = subst_cterm tau_cterm s :=
         (ext_cterm sigma_cterm tau_cterm Eq_cterm s3)
         (ext_cterm sigma_cterm tau_cterm Eq_cterm s4)
         (ext_cterm sigma_cterm tau_cterm Eq_cterm s5)
+  | pbool => congr_pbool
+  | ptrue => congr_ptrue
+  | pfalse => congr_pfalse
+  | pif s0 s1 s2 s3 =>
+      congr_pif (ext_cterm sigma_cterm tau_cterm Eq_cterm s0)
+        (ext_cterm sigma_cterm tau_cterm Eq_cterm s1)
+        (ext_cterm sigma_cterm tau_cterm Eq_cterm s2)
+        (ext_cterm sigma_cterm tau_cterm Eq_cterm s3)
   end.
 
 Lemma up_ren_ren_cterm_cterm (xi : nat -> nat) (zeta : nat -> nat)
@@ -626,6 +694,14 @@ ren_cterm zeta_cterm (ren_cterm xi_cterm s) = ren_cterm rho_cterm s :=
         (compRenRen_cterm xi_cterm zeta_cterm rho_cterm Eq_cterm s3)
         (compRenRen_cterm xi_cterm zeta_cterm rho_cterm Eq_cterm s4)
         (compRenRen_cterm xi_cterm zeta_cterm rho_cterm Eq_cterm s5)
+  | pbool => congr_pbool
+  | ptrue => congr_ptrue
+  | pfalse => congr_pfalse
+  | pif s0 s1 s2 s3 =>
+      congr_pif (compRenRen_cterm xi_cterm zeta_cterm rho_cterm Eq_cterm s0)
+        (compRenRen_cterm xi_cterm zeta_cterm rho_cterm Eq_cterm s1)
+        (compRenRen_cterm xi_cterm zeta_cterm rho_cterm Eq_cterm s2)
+        (compRenRen_cterm xi_cterm zeta_cterm rho_cterm Eq_cterm s3)
   end.
 
 Lemma up_ren_subst_cterm_cterm (xi : nat -> nat) (tau : nat -> cterm)
@@ -722,6 +798,15 @@ subst_cterm tau_cterm (ren_cterm xi_cterm s) = subst_cterm theta_cterm s :=
         (compRenSubst_cterm xi_cterm tau_cterm theta_cterm Eq_cterm s3)
         (compRenSubst_cterm xi_cterm tau_cterm theta_cterm Eq_cterm s4)
         (compRenSubst_cterm xi_cterm tau_cterm theta_cterm Eq_cterm s5)
+  | pbool => congr_pbool
+  | ptrue => congr_ptrue
+  | pfalse => congr_pfalse
+  | pif s0 s1 s2 s3 =>
+      congr_pif
+        (compRenSubst_cterm xi_cterm tau_cterm theta_cterm Eq_cterm s0)
+        (compRenSubst_cterm xi_cterm tau_cterm theta_cterm Eq_cterm s1)
+        (compRenSubst_cterm xi_cterm tau_cterm theta_cterm Eq_cterm s2)
+        (compRenSubst_cterm xi_cterm tau_cterm theta_cterm Eq_cterm s3)
   end.
 
 Lemma up_subst_ren_cterm_cterm (sigma : nat -> cterm)
@@ -829,6 +914,15 @@ ren_cterm zeta_cterm (subst_cterm sigma_cterm s) = subst_cterm theta_cterm s
         (compSubstRen_cterm sigma_cterm zeta_cterm theta_cterm Eq_cterm s3)
         (compSubstRen_cterm sigma_cterm zeta_cterm theta_cterm Eq_cterm s4)
         (compSubstRen_cterm sigma_cterm zeta_cterm theta_cterm Eq_cterm s5)
+  | pbool => congr_pbool
+  | ptrue => congr_ptrue
+  | pfalse => congr_pfalse
+  | pif s0 s1 s2 s3 =>
+      congr_pif
+        (compSubstRen_cterm sigma_cterm zeta_cterm theta_cterm Eq_cterm s0)
+        (compSubstRen_cterm sigma_cterm zeta_cterm theta_cterm Eq_cterm s1)
+        (compSubstRen_cterm sigma_cterm zeta_cterm theta_cterm Eq_cterm s2)
+        (compSubstRen_cterm sigma_cterm zeta_cterm theta_cterm Eq_cterm s3)
   end.
 
 Lemma up_subst_subst_cterm_cterm (sigma : nat -> cterm)
@@ -938,6 +1032,15 @@ subst_cterm tau_cterm (subst_cterm sigma_cterm s) = subst_cterm theta_cterm s
         (compSubstSubst_cterm sigma_cterm tau_cterm theta_cterm Eq_cterm s3)
         (compSubstSubst_cterm sigma_cterm tau_cterm theta_cterm Eq_cterm s4)
         (compSubstSubst_cterm sigma_cterm tau_cterm theta_cterm Eq_cterm s5)
+  | pbool => congr_pbool
+  | ptrue => congr_ptrue
+  | pfalse => congr_pfalse
+  | pif s0 s1 s2 s3 =>
+      congr_pif
+        (compSubstSubst_cterm sigma_cterm tau_cterm theta_cterm Eq_cterm s0)
+        (compSubstSubst_cterm sigma_cterm tau_cterm theta_cterm Eq_cterm s1)
+        (compSubstSubst_cterm sigma_cterm tau_cterm theta_cterm Eq_cterm s2)
+        (compSubstSubst_cterm sigma_cterm tau_cterm theta_cterm Eq_cterm s3)
   end.
 
 Lemma renRen_cterm (xi_cterm : nat -> nat) (zeta_cterm : nat -> nat)
@@ -1089,6 +1192,14 @@ Fixpoint rinst_inst_cterm (xi_cterm : nat -> nat)
         (rinst_inst_cterm xi_cterm sigma_cterm Eq_cterm s3)
         (rinst_inst_cterm xi_cterm sigma_cterm Eq_cterm s4)
         (rinst_inst_cterm xi_cterm sigma_cterm Eq_cterm s5)
+  | pbool => congr_pbool
+  | ptrue => congr_ptrue
+  | pfalse => congr_pfalse
+  | pif s0 s1 s2 s3 =>
+      congr_pif (rinst_inst_cterm xi_cterm sigma_cterm Eq_cterm s0)
+        (rinst_inst_cterm xi_cterm sigma_cterm Eq_cterm s1)
+        (rinst_inst_cterm xi_cterm sigma_cterm Eq_cterm s2)
+        (rinst_inst_cterm xi_cterm sigma_cterm Eq_cterm s3)
   end.
 
 Lemma rinstInst'_cterm (xi_cterm : nat -> nat) (s : cterm) :
@@ -1341,6 +1452,13 @@ Fixpoint allfv_cterm (p_cterm : nat -> Prop) (s : cterm) {struct s} : Prop :=
               (and (allfv_cterm p_cterm s3)
                  (and (allfv_cterm p_cterm s4)
                     (and (allfv_cterm p_cterm s5) True)))))
+  | pbool => True
+  | ptrue => True
+  | pfalse => True
+  | pif s0 s1 s2 s3 =>
+      and (allfv_cterm p_cterm s0)
+        (and (allfv_cterm p_cterm s1)
+           (and (allfv_cterm p_cterm s2) (and (allfv_cterm p_cterm s3) True)))
   end.
 
 Lemma upAllfvTriv_cterm_cterm {p : nat -> Prop} (H : forall x, p x) :
@@ -1418,6 +1536,14 @@ allfv_cterm p_cterm s :=
               (conj (allfvTriv_cterm p_cterm H_cterm s3)
                  (conj (allfvTriv_cterm p_cterm H_cterm s4)
                     (conj (allfvTriv_cterm p_cterm H_cterm s5) I)))))
+  | pbool => I
+  | ptrue => I
+  | pfalse => I
+  | pif s0 s1 s2 s3 =>
+      conj (allfvTriv_cterm p_cterm H_cterm s0)
+        (conj (allfvTriv_cterm p_cterm H_cterm s1)
+           (conj (allfvTriv_cterm p_cterm H_cterm s2)
+              (conj (allfvTriv_cterm p_cterm H_cterm s3) I)))
   end.
 
 Lemma upAllfvImpl_cterm_cterm {p : nat -> Prop} {q : nat -> Prop}
@@ -1730,6 +1856,47 @@ allfv_cterm p_cterm s -> allfv_cterm q_cterm s :=
                                   end
                               end
                           end) I)))))
+  | pbool => fun HP => I
+  | ptrue => fun HP => I
+  | pfalse => fun HP => I
+  | pif s0 s1 s2 s3 =>
+      fun HP =>
+      conj
+        (allfvImpl_cterm p_cterm q_cterm H_cterm s0
+           match HP with
+           | conj HP _ => HP
+           end)
+        (conj
+           (allfvImpl_cterm p_cterm q_cterm H_cterm s1
+              match HP with
+              | conj _ HP => match HP with
+                             | conj HP _ => HP
+                             end
+              end)
+           (conj
+              (allfvImpl_cterm p_cterm q_cterm H_cterm s2
+                 match HP with
+                 | conj _ HP =>
+                     match HP with
+                     | conj _ HP => match HP with
+                                    | conj HP _ => HP
+                                    end
+                     end
+                 end)
+              (conj
+                 (allfvImpl_cterm p_cterm q_cterm H_cterm s3
+                    match HP with
+                    | conj _ HP =>
+                        match HP with
+                        | conj _ HP =>
+                            match HP with
+                            | conj _ HP =>
+                                match HP with
+                                | conj HP _ => HP
+                                end
+                            end
+                        end
+                    end) I)))
   end.
 
 Lemma upAllfvRenL_cterm_cterm (p : nat -> Prop) (xi : nat -> nat) :
@@ -2036,6 +2203,45 @@ allfv_cterm (funcomp p_cterm xi_cterm) s :=
                                   end
                               end
                           end) I)))))
+  | pbool => fun H => I
+  | ptrue => fun H => I
+  | pfalse => fun H => I
+  | pif s0 s1 s2 s3 =>
+      fun H =>
+      conj
+        (allfvRenL_cterm p_cterm xi_cterm s0 match H with
+                                             | conj H _ => H
+                                             end)
+        (conj
+           (allfvRenL_cterm p_cterm xi_cterm s1
+              match H with
+              | conj _ H => match H with
+                            | conj H _ => H
+                            end
+              end)
+           (conj
+              (allfvRenL_cterm p_cterm xi_cterm s2
+                 match H with
+                 | conj _ H =>
+                     match H with
+                     | conj _ H => match H with
+                                   | conj H _ => H
+                                   end
+                     end
+                 end)
+              (conj
+                 (allfvRenL_cterm p_cterm xi_cterm s3
+                    match H with
+                    | conj _ H =>
+                        match H with
+                        | conj _ H =>
+                            match H with
+                            | conj _ H => match H with
+                                          | conj H _ => H
+                                          end
+                            end
+                        end
+                    end) I)))
   end.
 
 Lemma upAllfvRenR_cterm_cterm (p : nat -> Prop) (xi : nat -> nat) :
@@ -2342,6 +2548,45 @@ allfv_cterm p_cterm (ren_cterm xi_cterm s) :=
                                   end
                               end
                           end) I)))))
+  | pbool => fun H => I
+  | ptrue => fun H => I
+  | pfalse => fun H => I
+  | pif s0 s1 s2 s3 =>
+      fun H =>
+      conj
+        (allfvRenR_cterm p_cterm xi_cterm s0 match H with
+                                             | conj H _ => H
+                                             end)
+        (conj
+           (allfvRenR_cterm p_cterm xi_cterm s1
+              match H with
+              | conj _ H => match H with
+                            | conj H _ => H
+                            end
+              end)
+           (conj
+              (allfvRenR_cterm p_cterm xi_cterm s2
+                 match H with
+                 | conj _ H =>
+                     match H with
+                     | conj _ H => match H with
+                                   | conj H _ => H
+                                   end
+                     end
+                 end)
+              (conj
+                 (allfvRenR_cterm p_cterm xi_cterm s3
+                    match H with
+                    | conj _ H =>
+                        match H with
+                        | conj _ H =>
+                            match H with
+                            | conj _ H => match H with
+                                          | conj H _ => H
+                                          end
+                            end
+                        end
+                    end) I)))
   end.
 
 End Allfv.
